Pushing up to Allocproof.v

backend/Cminor.v
@@ -615,6 +615,7 @@ Inductive entry_point (p: program): mem -> state -> val -> list val -> Prop :=
       Mem.arg_well_formed args m0 ->
       globals_not_fresh ge m0 ->
       Genv.find_funct_ptr ge b = Some f ->
+      Val.has_type_list args (sig_args (funsig f)) ->
       entry_point p m0 (Callstate f args Kstop m0) fp args.
 
 (** A final state is a [Returnstate] with an empty continuation. *)
@@ -1229,6 +1230,7 @@ Proof.
   + constructor.
   + unfold globals_not_fresh.
     erewrite Genv.init_mem_genv_next; eauto; reflexivity.
+  + rewrite H3; simpl; auto.
   + split. apply eval_funcall_steps. eauto. red; auto.
   econstructor.
 -(* divergence *)
@@ -1239,6 +1241,7 @@ Proof.
          constructor.
          unfold globals_not_fresh.
          erewrite Genv.init_mem_genv_next; eauto; reflexivity.
+         rewrite H3; simpl; auto.
   eapply forever_plus_forever.
   eapply evalinf_funcall_forever; eauto.
 Qed.
