cfrontend/Cshmgen.v
@@ -697,3 +697,4 @@ Definition transl_globvar (id: ident) (ty: type) := OK tt.
 Definition transl_program (p: Clight.program) : res program :=
   transform_partial_program2 (transl_fundef p.(prog_comp_env)) transl_globvar p.
 
+ 
